Prototype linear environment in sat

theories/Map.v
@@ -8,10 +8,44 @@ Module Env <: FMapInterface.S := FMapAVL.Make OrderedTypeEx.Nat_as_OT.
 
 Definition map := Env.t.
 
-Definition empty {V}: Env.t V := Env.empty _.
-Definition add {V}: nat -> V -> Env.t V -> Env.t V := @Env.add _.
-Definition merge {V}: Env.t V -> Env.t V -> Env.t V := Env.map2 (fun x y => if x is Some _ then x else y).
+Definition empty {V}: map V := Env.empty _.
+Definition add {V}: nat -> V -> map V -> map V := @Env.add _.
+Definition merge {V}: map V -> map V -> map V := Env.map2 (fun x y => if x is Some _ then x else y).
 
-Definition one {V} (x: nat) (v: V) := Env.add x v (Env.empty _).
-Definition minus {V}: nat -> Env.t V -> Env.t V := @Env.remove _.
-Definition find {V}: nat -> Env.t V -> option V := @Env.find _.
+Definition one {V} (x: nat) (v: V) := add x v empty.
+Definition minus {V}: nat -> map V -> map V := @Env.remove _.
+Definition find {V}: nat -> map V -> option V := @Env.find _.
+
+Lemma add_minus {V}:
+  forall x (t: V) Γ,
+    find x Γ = Some t ->
+    add x t (minus x Γ) = Γ.
+Proof.
+  intros x t Γ p.
+  unfold add, minus.
+  admit.
+Admitted.
+
+Lemma find_add {V}:
+  forall x (t: V) Γ,
+    find x (add x t Γ) = Some t.
+Proof.
+  intros x t.
+  admit.
+Admitted.
+
+Lemma always_empty {V}:
+  forall x (t: V), Env.is_empty (minus x (add x t empty)) = true.
+Proof.
+  intros ? ?.
+  unfold one.
+  admit.
+Admitted.
+
+Lemma remove_add {V}:
+  forall x (t: V) Γ,
+    minus x (add x t Γ) = Γ.
+Proof.
+  intros x t.
+  admit.
+Admitted.
